

1. Consider $dx_t = f(x_t, t) dt + g(x_t, t) dW_t$

with Fokker Planck equation

$$\frac{\partial}{\partial t} p = -\frac{\partial}{\partial x}(f p) + \frac{1}{2} \frac{\partial^2}{\partial x^2}(g^2 p) \quad - (1)$$

We want to find $v(x, t)$ such that $d(x_t) = v(x_t, t) dt$

$$\text{Since } \frac{\partial p}{\partial t} = -\frac{\partial}{\partial x}(v p)$$

$$\text{By (1), } \frac{\partial}{\partial x}(v p) = \frac{\partial}{\partial x}(f p) - \frac{1}{2} \frac{\partial^2}{\partial x^2}(g^2 p)$$

$$\Rightarrow v p = f p - \frac{1}{2} \frac{\partial}{\partial x}(g^2 p)$$

$$v = f - \frac{1}{2} \frac{1}{p} \frac{\partial}{\partial x}(g^2 p)$$

$$v = f - \frac{1}{2} (\partial_x g^2) - \frac{1}{2} g^2 \frac{\partial p}{p}$$

$$\text{By } \frac{\partial x p}{p} = \partial x / g p, \quad v(x, t) = f(x_t, t) - \frac{1}{2} \frac{\partial}{\partial x} g^2(x_t, t) - \frac{g^2(x_t, t)}{2} \frac{\partial}{\partial x} \ln p(x_t, t)$$

$$dx_t = \left(f(x_t, t) - \frac{1}{2} \frac{\partial}{\partial x} g^2(x_t, t) - \frac{g^2(x_t, t)}{2} \frac{\partial}{\partial x} \ln p(x_t, t) \right) dt$$

2. 詳見 problem 2.pdf

3. Unanswered Question:

Can Backward SDE actually back to initial data distribution in practice?